LeanLambdaLibMathlib/LambdaLib/progtests.lean
@@ -1,0 +1,134 @@
+import LambdaLib.qterm
+import LambdaLib.unification
+import LambdaLib.functions.pmatch
+import LambdaLib.functions.prog
+-- import Mathlib.Tactic
+
+-- this file has test cases that i need to work for the embedding
+-- to eventually work
+
+open QuotTerm
+
+namespace S
+abbrev pair := <λ t1 t2 p. p t1 t2>
+abbrev proj1 := <λ p. p (λ x y. x)>
+abbrev proj2 := <λ p. p (λ x y. y)>
+-- TODO: i can make syntax for pair with a macro, which will run before the elaborator!
+
+-- contexts
+abbrev nil := <Nil>
+abbrev cons := <λ ctx lvl ty. Cons ctx lvl ty>
+
+-- variables
+abbrev zero := <λ env. {proj2} env>
+abbrev succ := <λ x env. x ({proj1} env)>
+
+abbrev pi := <λ x y env. Pi (x env) (λ a. y ({pair} env a))>
+abbrev U := <λ env. U>
+abbrev Empty := <λ env. Empty>
+abbrev Lift := <λ T env. Lift (T env)>
+end S
+
+noncomputable def means_prog (prev : QTerm → Option (QTerm → Prop))
+  (ty : QTerm) : Prog QTerm (QTerm → Prop) :=
+  Pmatch2
+    (fun A B ↦ ty = <Pi {A} {B}>)
+    (fun A B => .Rec PUnit (fun _ => A)
+      (fun mA => .Rec {a // mA .unit a} (fun ⟨a, _aInA⟩ ↦ <{B} {a}>)
+      (fun mBa ↦ .Ret (some
+        (fun f ↦ ∀ (a : QTerm) (inA : mA .unit a), mBa ⟨a, inA⟩ <{f} {a}>)))))
+  (Pif (ty = <U>)
+    (.Ret (some (fun T ↦ ∃ S, prev T = some S)))
+    -- (.Ret (recorder prev))
+    -- catchall case shouldn't happen
+    (.Ret .none))
+
+noncomputable def means'
+  (prev : QTerm → Option (QTerm → Prop))
+  (ty : QTerm)
+  : Option (QTerm → Prop)
+  := runProg (means_prog prev) ty
+
+noncomputable def means (lvl : Nat) (ty : QTerm) : Option (QTerm → Prop) :=
+  match lvl with
+  | .zero => none -- some (fun _ ↦ False)
+  -- | .succ lvl' => means' (means lvl') ty
+  | .succ lvl' => runProg (means_prog (means lvl')) ty
+
+example (SA SB A B)
+  (rec1 : means 1 A = some SA)
+  (rec2 : means 1 B = some SB)
+  : means 1 <Pi {A} (λ a. {B})> = some (fun f ↦ ∀ a, SA a → SB <{f} {a}>)
+  := by
+  --
+  repeat (first
+    | simp only [means, means', means_prog]
+    | simp only [runProg, runProgDefinitionRet, runProgDefinitionRec, collectOptionDef]
+    | simp (disch := intros; lambda_solve; try trivial) only [PmatchDef1, PmatchDef2]
+    | simp (disch := intros; lambda_solve; try trivial) only [Pmatch2Def1, Pmatch2Def2]
+    | simp (disch := intros; lambda_solve; try trivial) only [PifDef1, PifDef2]
+  )
+  --
+  simp only [means, means', means_prog, runProg,
+    runProgDefinitionRet, runProgDefinitionRec, collectOptionDef] at rec1
+  --
+  -- rewrite [rec1]
+  rewrite [rec1]
+  --
+  simp only [means, means', means_prog, runProg,
+    runProgDefinitionRet, runProgDefinitionRec, collectOptionDef] at rec2
+  normalize
+  --
+  rewrite [rec2]
+  clear rec1 rec2
+  simp only [collectOptionDef, mybindDef1]
+  --
+
+macro "normalize2" : tactic => `(tactic|
+  simp only [lift_app, lift_lam, lift_var, lift_const,
+      subst_app, subst_lam, subst_var, subst_const,
+      liftLiftMulti, substLiftMulti, liftMultiZero,
+      liftMulti_lam_rw, liftMulti_app_rw, liftMulti_var_rw, liftMulti_const_rw,
+      beta] at *
+)
+
+macro "lambda_solve2" : tactic => `(tactic|
+  repeat ( first
+    | trivial
+    -- | simp at * -- TODO: figure out which lemmas this is using (relating to ∧) and write explicitly
+    -- | normalize2
+    -- | simp only [lam_body_rw, const_inj_rw, var_inj_rw, var_not_const_rw, var_not_const_rw2] at *
+    -- | simp (disch := repeat constructor) only [app_fact_rw, app_ne_const_rw, app_ne_var_rw] at *
+    | fail_if_no_progress subst_vars -- TODO: maybe only have this go on equations of type QTerm
+    | casesm* _ ∧ _, QTerm × QTerm
+    | simp [*] -- TODO: maybe i can use the `contextual' flag instead
+  )
+)
+
+-- this one was giving more trouble in embedding.lean
+example {mty env} {lvl : Nat}
+  (H : means lvl.succ.succ (< {S.U} {env} >) = some mty)
+  : False
+  := by
+  --
+  -- the clear H makes it run fast instead of slow
+  repeat (first
+    | simp only [means, means', means_prog, runProg, runProgDefinitionRet,
+      runProgDefinitionRec, collectOptionDef] at H
+    | simp (disch := clear H; intros; lambda_solve; try trivial) only
+      [PmatchDef1, PmatchDef2, Pmatch2Def1, Pmatch2Def2, PifDef1, PifDef2] at H
+  )
+  --
+  simp only [means, means', means_prog, runProg,
+    runProgDefinitionRet, runProgDefinitionRec, collectOptionDef] at H
+  --
+  -- lambda_solve
+  --
+  simp (disch := clear H; intros; lambda_solve; try trivial) only
+    [PmatchDef1, PmatchDef2, Pmatch2Def1, Pmatch2Def2, PifDef1, PifDef2] at H
+  --
+  simp (disch := intros; lambda_solve; try trivial) only [PifDef1, PifDef2] at H
+  -- this is now slow again.......
+  simp (disch := intros; lambda_solve; try trivial) only [Pmatch2Def1, Pmatch2Def2] at H
+  --
+  sorry
